lenient_wp rule for framing operand stack

theories/iris/language/lenient_wp.v
@@ -67,7 +67,7 @@ Section lenient_wp.
     (∀ f, lp_trap Ψ ∗ lp_fr Ψ f -∗ lp_trap Φ ∗ lp_fr Φ f) ∗
     (* non-trap case: old frame and non-trap conditions imply the new wp *)
     (∀ w f, lp_notrap Ψ w ∗ ↪[frame] f ∗ lp_fr Ψ f -∗ lenient_wp s E (of_val w ++ es2) Φ)
-    ⊢ lenient_wp s E (es1 ++ es2) (Φ).
+    ⊢ lenient_wp s E (es1 ++ es2) Φ.
   Proof.
     iIntros "(Hes1 & Htrapimpl & Hes2)".
     iApply (wp_seq_can_trap s E _ (lp_notrap Ψ) _ _ Ψ.(lp_fr) (↪[BAIL] ∗ Ψ.(lp_trap))).
@@ -90,6 +90,73 @@ Section lenient_wp.
     - iIntros (w f) "(Hnotrap & Hfr & Hfrcond)".
       iApply "Hes2".
       iFrame.
+  Qed.
+
+
+  Definition sigT_apply {A} {P: A -> Type} (f: forall a, P a -> P a) (x: {a: A & P a}) : {a: A & P a} :=
+    existT (projT1 x) (f _ (projT2 x)).
+
+  (* This is like composition with val_combine *)
+  Definition lp_combine {A} (l: logp A) vs : logp A :=
+    {|
+      lp_fr := lp_fr l;
+      lp_val vs' := lp_val l (seq.cat vs vs');
+      lp_trap := lp_trap l;
+      lp_br vh := lp_br l (sigT_apply (λ _ vh0, vh_push_const vh0 vs) vh);
+      lp_ret lh := lp_ret l (sh_push_const lh vs);
+      lp_host tf h cvs sh := lp_host l tf h cvs (llh_push_const sh vs);
+    |}.
+
+  Lemma lp_combine_val:
+    forall (Φ: logpred) vs w,
+      (denote_logpred Φ) (val_combine (immV vs) w) ⊣⊢ denote_logpred (lp_combine Φ vs) w.
+  Proof.
+    intros Φ vs w.
+    unfold lp_combine, val_combine, denote_logpred, lp_noframe.
+    cbn.
+    by destruct w.
+  Qed.
+
+  Lemma lp_expand Φ w:
+    denote_logpred Φ w ⊣⊢ (⌜w = trapV⌝ ∗ ↪[BAIL] ∗ lp_trap Φ ∨ lp_notrap Φ w) ∗ ∃ f, ↪[frame] f ∗ lp_fr Φ f.
+  Proof.
+    destruct w;
+      unfold denote_logpred, lp_noframe;
+      iSplit;
+      cbn;
+      iIntros "[Hpost Hfr]";
+      iFrame.
+    - by iDestruct "Hpost" as "[[%Hcontra _] | Hpost]".
+    - iLeft. by iFrame.
+    - iDestruct "Hpost" as "[[_ Hpost] | %Hcontra]"; [iFrame|by exfalso].
+    - by iDestruct "Hpost" as "[[%Hcontra _] | Hpost]".
+    - by iDestruct "Hpost" as "[[%Hcontra _] | Hpost]".
+    - by iDestruct "Hpost" as "[[%Hcontra _] | Hpost]".
+  Qed.
+
+  Lemma lenient_wp_val_cons s E (Φ: logpred) v es :
+    lenient_wp NotStuck E es (lp_combine Φ [v])
+    ⊢ lenient_wp s E (AI_basic (BI_const v) :: es) Φ.
+  Proof.
+    iIntros "Hcomb".
+    iApply (wp_wand with "[Hcomb]").
+    - iApply (wp_val_can_trap_precise _ _ (lp_notrap Φ) _ _ (lp_fr Φ) (lp_trap Φ ∗ ↪[BAIL])).
+      iSplitR; [done|].
+      unfold lenient_wp.
+      iApply (wp_wand with "[Hcomb]").
+      iApply "Hcomb".
+      iIntros (w) "Hden".
+      setoid_rewrite <- lp_combine_val at 1.
+      setoid_rewrite -> lp_expand at 1.
+      iDestruct "Hden" as "[[(%Hcomb & Hbail & Htrap) | Hnotrap] Hfr]";
+        iFrame.
+      iLeft.
+      iFrame.
+      iPureIntro.
+      destruct w; vm_compute in Hcomb; congruence.
+    - iIntros (w) "[[(%Hcomb & Hbail & Htrap) | Hnotrap] Hfr]";
+        rewrite lp_expand; iFrame.
+      iLeft; by iFrame.
   Qed.
 
 End lenient_wp.
